Only small admits in SpecProperties

proof/spec/KyberProperties.ec
@@ -76,6 +76,27 @@ phoare sem_decode10_vec a : [ EncDec.decode10_vec : arg = a ==> res = sem_decode
 phoare sem_encode12_vec a : [ EncDec.encode12_vec : arg = a ==> res = sem_encode12_vec a ] = 1%r by admit. (* reify *)
 phoare sem_encode10_vec a : [ EncDec.encode10_vec : arg = a ==> res = sem_encode10_vec a ] = 1%r by admit. (* reify *)
 
+(****** TO DO WE NEED THESE Lemmas HERE *********)
+
+axiom invnttK : cancel ntt invntt.
+axiom nttK : cancel invntt ntt.
+axiom nttvK : cancel invnttv nttv.
+axiom invnttvK : cancel nttv invnttv.
+axiom nttmK : cancel invnttm nttm.
+axiom invnttmK : cancel nttm invnttm.
+axiom mul_comm_ntt (pa pb : poly):
+  ntt (pa &* pb) = basemul (ntt pa) (ntt pb).
+axiom add_comm_ntt (pa pb : poly):
+  ntt (pa &+ pb) = (ntt pa) &+ (ntt pb).
+axiom add_comm_invntt (pa pb : poly) : 
+  invntt (pa &+ pb) = (invntt pa) &+ (invntt pb).
+axiom mul_comm_invntt(pa pb : poly) :
+  invntt (basemul pa  pb) = (invntt pa) &* (invntt pb).
+axiom nttZero : ntt KPoly.zero = KPoly.zero.
+
+(************************************************)
+
+
 (**************************************************************************
    MLWE_PKE is the theory where we prove an abstract PKE construction
    that matches the algebraic basis of Kyber. This theory clones MLWE
@@ -105,10 +126,10 @@ type pkey = W8.t Array1152.t * W8.t Array32.t.
 type skey = W8.t Array1152.t.  
 
 op pk_encode(pk : vector * W8.t Array32.t) : pkey = 
-                                  (sem_encode12_vec (toipolyvec pk.`1) ,pk.`2).
-op pk_decode(pk : pkey) = (ofipolyvec (sem_decode12_vec pk.`1) ,pk.`2).
-op sk_encode(sk : vector) : skey = sem_encode12_vec (toipolyvec sk).
-op sk_decode(sk : skey) = ofipolyvec (sem_decode12_vec sk).
+                                  (sem_encode12_vec (toipolyvec (nttv pk.`1)) ,pk.`2).
+op pk_decode(pk : pkey) = (invnttv (ofipolyvec (sem_decode12_vec (pk.`1))),pk.`2).
+op sk_encode(sk : vector) : skey = sem_encode12_vec (toipolyvec (nttv sk)).
+op sk_decode(sk : skey) = invnttv (ofipolyvec (sem_decode12_vec sk)).
 op m_encode(m : plaintext) : poly = decompress_poly 1 (sem_decode1 m).
 op m_decode(p : poly) : plaintext = sem_encode1 (compress_poly 1 p). 
 op c_encode(c :  vector * poly) : ciphertext = 
@@ -207,12 +228,12 @@ clone import MLWE_PKE as MLWEPKE with
 
 realize pk_encodeK.
 rewrite /pk_decode /pk_encode /cancel /= => x.
-by rewrite sem_encode12_vecK toipolyvecK /#.
+by rewrite sem_encode12_vecK toipolyvecK invnttvK /#.
 qed.
 
 realize sk_encodeK.
 rewrite /sk_decode /sk_encode /cancel /= => x.
-by rewrite sem_encode12_vecK toipolyvecK /#.
+rewrite sem_encode12_vecK toipolyvecK invnttvK /#.
 qed.
 
 realize encode_noise.
@@ -356,49 +377,65 @@ syntactic reasons in the following proof
 steps.
 *************************************)
 
-module type NoiseSampler = {
-  proc sample2(noiseseed:W8.t Array32.t) : vector * vector * int
+module type NoiseSampler(PRF1 : PRF_.PseudoRF, PRF2 : PRF_.PseudoRF) = {
+  proc sample2(noiseseed:W8.t Array32.t) : vector * vector
   proc sample3(noiseseed:W8.t Array32.t) : vector * vector * poly
 }.
 
 
-module KNS : NoiseSampler = {
-  proc sample2(noiseseed:W8.t Array32.t) : vector * vector * int= {
+module (KNS : NoiseSampler) (PRF1 : PRF_.PseudoRF, PRF2 : PRF_.PseudoRF) = {
+  proc sample2(noiseseed:W8.t Array32.t) : vector * vector = {
     var noise1, noise2, _N,i,c;
     noise1 <- witness;                     
     noise2 <- witness;                      
     _N <- 0;                      
     i <- 0;                             
     while (i < kvec) {                 
-      c <@ CBD2(KPRF).sample(noiseseed,_N);
+      c <@ CBD2(PRF1).sample(noiseseed,_N);
       noise1 <- set noise1 i c;                   
       _N <- _N + 1;                     
      i <- i + 1;                       
     }                                  
     i <- 0;                             
     while (i < kvec) {                 
-      c <@ CBD2(KPRF).sample(noiseseed,_N);
+      c <@ CBD2(PRF1).sample(noiseseed,_N);
       noise2 <- set noise2 i c;                   
       _N <- _N + 1;                     
       i <- i + 1;                       
     }                                  
 
-    return (noise1,noise2,_N);
+    return (noise1,noise2);
   }
 
    proc sample3(noiseseed:W8.t Array32.t) : vector * vector * poly = {
-     var e, s, _N,e2;
-     (s,e,_N) <@ sample2(noiseseed);
-     e2 <@ CBD2(KPRF).sample(noiseseed,_N);
-     return (s,e, e2);
+     var e2,noise1, noise2, _N,i,c;
+     noise1 <- witness;                     
+     noise2 <- witness;                      
+     _N <- 0;                      
+     i <- 0;                             
+     while (i < kvec) {                 
+       c <@ CBD2(PRF2).sample(noiseseed,_N);
+       noise1 <- set noise1 i c;                   
+       _N <- _N + 1;                     
+      i <- i + 1;                       
+     }                                  
+     i <- 0;                             
+     while (i < kvec) {                 
+       c <@ CBD2(PRF2).sample(noiseseed,_N);
+      noise2 <- set noise2 i c;                   
+      _N <- _N + 1;                     
+      i <- i + 1;                       
+     }                                  
+     e2 <@ CBD2(PRF2).sample(noiseseed,_N);
+     return (noise1,noise2, e2);
   }
 }.
 
-module KyberS(HS : HSF.PseudoRF, S : Sampler, NS : NoiseSampler, PRF : PRF_.PseudoRF, O : RO.POracle) : Scheme = {
+module KyberS(HS : HSF.PseudoRF, S : Sampler, NS : NoiseSampler, PRF1 : PRF_.PseudoRF, PRF2 : PRF_.PseudoRF, O : RO.POracle) : Scheme = {
 
   (* Spec gives a derandomized enc that matches this code *)
   proc kg_derand(rho sig: W8.t Array32.t) : pkey * skey = {
-     var _N,t;
+     var t;
      var tv,sv : W8.t Array1152.t;
      var a : matrix;
      var s,e : vector;
@@ -407,7 +444,7 @@ module KyberS(HS : HSF.PseudoRF, S : Sampler, NS : NoiseSampler, PRF : PRF_.Pseu
      sv <- witness;
      tv <- witness;
      a <@ S(O).sampleA(rho);     
-     (s,e,_N) <@ NS.sample2(sig);
+     (s,e) <@ NS(PRF1,PRF2).sample2(sig);
      s <- nttv s;
      e <- nttv e; 
      t <- ntt_mmul a s + e;
@@ -439,7 +476,7 @@ module KyberS(HS : HSF.PseudoRF, S : Sampler, NS : NoiseSampler, PRF : PRF_.Pseu
       thati <@ EncDec.decode12_vec(tv); 
       that <- ofipolyvec thati;
       aT <@ S(O).sampleAT(rho);    
-      (rv,e1,e2) <@ NS.sample3(r);
+      (rv,e1,e2) <@ NS(PRF1,PRF2).sample3(r);
       rhat <- nttv rv;
       u <- invnttv (ntt_mmul aT rhat) + e1;
       mp <@ EncDec.decode1(m);
@@ -451,7 +488,7 @@ module KyberS(HS : HSF.PseudoRF, S : Sampler, NS : NoiseSampler, PRF : PRF_.Pseu
 
   proc enc(pk : pkey, m : plaintext) : ciphertext = {
      var r,c;
-     r <@ PRF.keygen();
+     r <@ PRF2.keygen();
      c <@ enc_derand(pk,m,r);
      return c;
   }
@@ -477,17 +514,17 @@ module KyberS(HS : HSF.PseudoRF, S : Sampler, NS : NoiseSampler, PRF : PRF_.Pseu
 
 (* We have that instantiating S with KSampler we get the Spec *)
 lemma kg_sampler_kg (O <: RO.POracle) (XOF <: XOF_t {-O}) :
-  equiv [   KyberS(KHS,KSampler(XOF),KNS,KPRF,O).kg ~ Kyber(KHS,XOF,KPRF,O).kg : 
+  equiv [   KyberS(KHS,KSampler(XOF),KNS,KPRF,KPRF,O).kg ~ Kyber(KHS,XOF,KPRF,O).kg : 
      ={arg} /\ ={glob O, glob XOF} ==> ={res, glob O, glob XOF}].
 proc;inline*. swap{1} 24 -8. swap{2} [4..5] 12.
 seq 18 13: (#pre /\ sig1{1} = sig{2} /\ rho1{1} = rho{2}  /\ 
-            a0{1} = a{2} /\ _N0{1} = _N{2} /\ sd{1} = rho{2}); 1: by  auto.
+            a0{1} = a{2} /\ _N{1} = _N{2} /\ sd{1} = rho{2}); 1: by  auto.
 by sim => />; wp; sim />.
 qed.
 
 lemma enc_sampler_enc (O <: RO.POracle)  (XOF <: XOF_t {-O}):
  equiv [
-   KyberS(KHS,KSampler(XOF),KNS,KPRF,O).enc ~ Kyber(KHS,XOF,KPRF,O).enc : 
+   KyberS(KHS,KSampler(XOF),KNS,KPRF,KPRF,O).enc ~ Kyber(KHS,XOF,KPRF,O).enc : 
     ={arg} /\ ={glob O, glob XOF} ==> ={res, glob O, glob XOF}].
 proc. 
 inline {1} 2; inline {2} 2. 
@@ -497,7 +534,7 @@ by inline *;sim />; wp; sim =>/> /#.
 qed.
 
 lemma enc_sampler_dec (O <: RO.POracle)  (XOF <: XOF_t) :
-  equiv [ KyberS(KHS,KSampler(XOF),KNS,KPRF,O).dec ~ Kyber(KHS,XOF,KPRF,O).dec : 
+  equiv [ KyberS(KHS,KSampler(XOF),KNS,KPRF,KPRF,O).dec ~ Kyber(KHS,XOF,KPRF,O).dec : 
      ={arg} /\ ={glob O} ==> ={res} ] by proc;inline *;sim => /#.
 
 (*******************************************************************)
@@ -511,52 +548,100 @@ clone import HS_DEFS.RF as IdealHSF with
    proof dR_ll by smt(dsmooth_ll).
 
 op [lossless funiform] dnbytes : W8.t Array128.t distr.
-clone import PRF_DEFS.RF as IdealPRF with
+clone import PRF_DEFS.RF as IdealPRF1 with
    op dR = fun (_: W8.t) => dnbytes
    proof dR_ll by smt(dnbytes_ll).
+
+clone import PRF_DEFS.RF as IdealPRF2 with
+   op dR = fun (_: W8.t) => dnbytes
+   proof dR_ll by smt(dnbytes_ll).
+
+module DummyHS_D(F : HS_DEFS.PRF_Oracles) = {
+   proc keygen() : W8.t Array32.t = { return witness;}
+   proc f(inp : W8.t Array32.t * unit) : W8.t Array64.t = { var out; out <@ F.f(); return out; }
+}.
 
 module DummyHS(F : HS_DEFS.PRF_Oracles) = {
    proc keygen() : W8.t Array32.t = { IdealHSF.RF.m <- SmtMap.empty; return witness;}
    proc f(inp : W8.t Array32.t * unit) : W8.t Array64.t = { var out; out <@ F.f(); return out; }
 }.
 
-module (D_ES(S : Sampler, NS : NoiseSampler, PRF : PRF_.PseudoRF, O : RO.Oracle, As : KyberPKE.AdversaryRO) : HS_DEFS.Distinguisher) (F : HS_DEFS.PRF_Oracles)  = {
+module (D_ES(S : Sampler, O : RO.Oracle, As : KyberPKE.AdversaryRO) : HS_DEFS.Distinguisher) (F : HS_DEFS.PRF_Oracles)  = {
 
     proc distinguish() : bool = {
        var b;
-       b <@ KyberPKE.CPAGameROM(KyberPKE.CPA,KyberS(DummyHS(F),S,KNS,KPRF),As,O).main();
+       b <@ KyberPKE.CPAGameROM(KyberPKE.CPA,KyberS(DummyHS_D(F),S,KNS,KPRF,KPRF),As,O).main();
        return b;
     } 
 }.
 
-module DummyPRF(F : PRF_DEFS.PRF_Oracles) = {
-   proc keygen() : W8.t Array32.t = { IdealHSF.RF.m <- SmtMap.empty; return witness;}
+module KyberSIdeal(HS : HSF.PseudoRF, S : Sampler, NS : NoiseSampler, PRF1 : PRF_.PseudoRF, PRF2 : PRF_.PseudoRF, O : RO.POracle) : Scheme = {
+
+  include KyberS(HS,S,NS,PRF1,PRF2,O) [-kg]
+
+  proc kg() : pkey * skey = {
+     var s,rho,sig,kp;
+     s <@ HS.keygen();
+     rho <$ srand;
+     sig <@ PRF1.keygen();
+     kp <@ kg_derand(rho,sig);
+     return kp;
+  }
+
+}.
+
+module DummyPRF1D(F : PRF_DEFS.PRF_Oracles) = {
+   proc keygen() : W8.t Array32.t = { return witness;}
    proc f(inp : W8.t Array32.t * W8.t) : W8.t Array128.t = { var out; out <@ F.f(inp.`2); return out; }
 }.
 
-module (D_PRF(S : Sampler, NS : NoiseSampler, O : RO.Oracle, As : KyberPKE.AdversaryRO) : PRF_DEFS.Distinguisher) (F : PRF_DEFS.PRF_Oracles)  = {
+module DummyPRF1(F : PRF_DEFS.PRF_Oracles) = {
+   proc keygen() : W8.t Array32.t = { IdealPRF1.RF.m <- SmtMap.empty; return witness;}
+   proc f(inp : W8.t Array32.t * W8.t) : W8.t Array128.t = { var out; out <@ F.f(inp.`2); return out; }
+}.
+
+module (D_PRF1(S : Sampler, O : RO.Oracle, As : KyberPKE.AdversaryRO) : PRF_DEFS.Distinguisher) (F : PRF_DEFS.PRF_Oracles)  = {
 
     proc distinguish() : bool = {
        var b;
-       b <@ KyberPKE.CPAGameROM(KyberPKE.CPA,KyberS(DummyHS(IdealHSF.RF),S,KNS,DummyPRF(F)),As,O).main();
+       b <@ KyberPKE.CPAGameROM(KyberPKE.CPA,KyberSIdeal(DummyHS(IdealHSF.RF),S,KNS,DummyPRF1(F),KPRF),As,O).main();
+       return b;
+    } 
+}.
+
+module DummyPRF2D(F : PRF_DEFS.PRF_Oracles) = {
+   proc keygen() : W8.t Array32.t = { return witness;}
+   proc f(inp : W8.t Array32.t * W8.t) : W8.t Array128.t = { var out; out <@ F.f(inp.`2); return out; }
+}.
+
+module DummyPRF2(F : PRF_DEFS.PRF_Oracles) = {
+   proc keygen() : W8.t Array32.t = { IdealPRF2.RF.m <- SmtMap.empty; return witness;}
+   proc f(inp : W8.t Array32.t * W8.t) : W8.t Array128.t = { var out; out <@ F.f(inp.`2); return out; }
+}.
+
+module (D_PRF2(S : Sampler, O : RO.Oracle, As : KyberPKE.AdversaryRO) : PRF_DEFS.Distinguisher) (F : PRF_DEFS.PRF_Oracles)  = {
+
+    proc distinguish() : bool = {
+       var b;
+       b <@ KyberPKE.CPAGameROM(KyberPKE.CPA,KyberSIdeal(DummyHS(IdealHSF.RF),S,KNS,DummyPRF1(IdealPRF1.RF),DummyPRF2D(F)),As,O).main();
        return b;
     } 
 }.
 
 section.
 
-declare module O <: RO.Oracle {-IdealHSF.RF, -KPRF, -B1ROM, -B2ROM, -HSF.PRF}.
-declare module S <: Sampler {-KPRF, -O, -B1ROM, -B2ROM}.
-declare module As <: KyberPKE.AdversaryRO {-IdealHSF.RF, -HSF.PRF, -O, -S, -KPRF, -B1ROM, -B2ROM}.
+declare module O <: RO.Oracle {-IdealPRF2.RF, -IdealPRF1.RF, -PRF_.PRF, -IdealHSF.RF, -KPRF, -B1ROM, -B2ROM, -HSF.PRF}.
+declare module S <: Sampler {-IdealPRF2.RF, -IdealPRF1.RF, -PRF_.PRF, -IdealHSF.RF, -KPRF, -O, -B1ROM, -B2ROM}.
+declare module As <: KyberPKE.AdversaryRO {-IdealPRF2.RF, -IdealPRF1.RF, -PRF_.PRF, -IdealHSF.RF, -HSF.PRF, -O, -S, -KPRF, -B1ROM, -B2ROM}.
 
 lemma ESHop &m :
-  Pr [ KyberPKE.CPAGameROM(KyberPKE.CPA,KyberS(KHS,S,KNS,KPRF),As,O).main() @ &m : res] -
-  Pr [ KyberPKE.CPAGameROM(KyberPKE.CPA,KyberS(DummyHS(IdealHSF.RF),S,KNS,KPRF),As,O).main() @ &m : res] = 
-  Pr [ HS_DEFS.IND(HSF.PRF,D_ES(S,KNS,KPRF,O,As)).main() @ &m : res ] - 
-  Pr [ HS_DEFS.IND(IdealHSF.RF,D_ES(S,KNS,KPRF,O,As)).main() @ &m : res ].
+  Pr [ KyberPKE.CPAGameROM(KyberPKE.CPA,KyberS(KHS,S,KNS,KPRF,KPRF),As,O).main() @ &m : res] -
+  Pr [ KyberPKE.CPAGameROM(KyberPKE.CPA,KyberS(DummyHS(IdealHSF.RF),S,KNS,KPRF,KPRF),As,O).main() @ &m : res] = 
+  Pr [ HS_DEFS.IND(HSF.PRF,D_ES(S,O,As)).main() @ &m : res ] - 
+  Pr [ HS_DEFS.IND(IdealHSF.RF,D_ES(S,O,As)).main() @ &m : res ].
 proof.
-have -> : Pr[CPAGameROM(CPA, KyberS(KHS, S, KNS, KPRF), As, O).main() @ &m : res]  = 
-          Pr[HS_DEFS.IND(HSF.PRF, D_ES(S, KNS, KPRF, O, As)).main() @ &m : res] .
+have -> : Pr[CPAGameROM(CPA, KyberS(KHS, S, KNS, KPRF,KPRF), As, O).main() @ &m : res]  = 
+          Pr[HS_DEFS.IND(HSF.PRF, D_ES(S, O, As)).main() @ &m : res] .
 + byequiv => //.
   proc. 
   inline {1} 2; inline {2} 2. inline {2} 2. inline {2} 3.
@@ -572,8 +657,8 @@ have -> : Pr[CPAGameROM(CPA, KyberS(KHS, S, KNS, KPRF), As, O).main() @ &m : res
   by sim.
 
 + have -> : 
-    Pr[CPAGameROM(CPA, KyberS(DummyHS(IdealHSF.RF), S, KNS, KPRF), As, O).main() @ &m : res] = 
-    Pr[HS_DEFS.IND(IdealHSF.RF, D_ES(S, KNS, KPRF, O, As)).main() @ &m : res].
+    Pr[CPAGameROM(CPA, KyberS(DummyHS(IdealHSF.RF), S, KNS, KPRF, KPRF), As, O).main() @ &m : res] = 
+    Pr[HS_DEFS.IND(IdealHSF.RF, D_ES(S, O, As)).main() @ &m : res].
 + byequiv => //.
   proc. 
   inline {1} 2; inline {2} 2. inline {2} 2. inline {2} 3.
@@ -591,25 +676,261 @@ have -> : Pr[CPAGameROM(CPA, KyberS(KHS, S, KNS, KPRF), As, O).main() @ &m : res
 done.
 qed.
 
-lemma PRFHop &m :
-  Pr [ KyberPKE.CPAGameROM(KyberPKE.CPA,KyberS(DummyHS(IdealHSF.RF),S,KNS,KPRF),As,O).main() @ &m : res] -
-  Pr [ KyberPKE.CPAGameROM(KyberPKE.CPA,KyberS(DummyHS(IdealHSF.RF),S,KNS,DummyPRF(IdealPRF.RF)),As,O).main() @ &m : res] = 
-  Pr [ PRF_DEFS.IND(PRF_.PRF,D_PRF(S,KNS,O,As)).main() @ &m : res ] - 
-  Pr [ PRF_DEFS.IND(IdealPRF.RF,D_PRF(S,KNS,O,As)).main() @ &m : res ].
-admitted.
-(* Need two hops *)
+lemma KyberS_KyberIdeal &m :
+  Pr [ KyberPKE.CPAGameROM(KyberPKE.CPA,KyberS(DummyHS(IdealHSF.RF),S,KNS,KPRF,KPRF),As,O).main() @ &m : res] =
+  Pr [ KyberPKE.CPAGameROM(KyberPKE.CPA,KyberSIdeal(DummyHS(IdealHSF.RF),S,KNS,KPRF,KPRF),As,O).main() @ &m : res].
+proof.
+byequiv => //.
+proc. 
+  inline {1} 2; inline {2} 2. 
+  wp; call(_: ={glob O}); 1: by sim.
+  wp; call(_: ={glob O, glob S}); 1: by sim.
+  rnd.
+  wp; call(_: ={glob O}); 1: by sim.
+  conseq (_: _ ==> ={pk, glob O,glob S}); 1: smt().
+  seq 1 1 : (={glob As, glob S, glob O}); 1: by sim.
+  inline {1} 1. inline {2} 1. 
+  wp; call(_: ={glob O, glob S}); 1: by sim.
+  conseq => />.
+  inline *.
+  rcondt{1} 6; 1: by move => *; auto => />;smt(@SmtMap).
+  seq {1} 5 2 : (true); 1: by auto.
+  wp.
+  conseq (_: _ ==> rho{2} = Array32.init (fun i => r{1}.[i]) /\ 
+                   k{2} = Array32.init (fun i => r{1}.[i+32]));
+  1: by move => /> [#] &1 r; 
+       rewrite !SmtMap.get_set_sameE !oget_some.
+  admit. (* Product of distributions *)
+qed.
+
+
+lemma PRFHop1 &m :
+  Pr [ KyberPKE.CPAGameROM(KyberPKE.CPA,KyberSIdeal(DummyHS(IdealHSF.RF),S,KNS,KPRF,KPRF),As,O).main() @ &m : res] -
+  Pr [ KyberPKE.CPAGameROM(KyberPKE.CPA,KyberSIdeal(DummyHS(IdealHSF.RF),S,KNS,DummyPRF1(IdealPRF1.RF),KPRF),As,O).main() @ &m : res] = 
+  Pr [ PRF_DEFS.IND(PRF_.PRF,D_PRF1(S,O,As)).main() @ &m : res ] - 
+  Pr [ PRF_DEFS.IND(IdealPRF1.RF,D_PRF1(S,O,As)).main() @ &m : res ].
+proof.
+have -> : Pr[CPAGameROM(CPA, KyberSIdeal(DummyHS(IdealHSF.RF), S, KNS, KPRF, KPRF), As, O).main() @ &m : res] = 
+          Pr[PRF_DEFS.IND(PRF_.PRF, D_PRF1(S, O, As)).main() @ &m : res].
++ byequiv => //.
+  proc. 
+  inline {1} 2; inline {2} 2. inline {2} 2. inline {2} 3.
+  wp; call(_: ={glob O}); 1: by sim.
+  wp; call(_: ={glob O, glob S}); 1: by sim.
+  rnd.
+  wp; call(_: ={glob O}); 1: by sim.
+  conseq (_: _ ==> ={pk, glob O,glob S}); 1: smt().
+  swap {2} 2 -1.
+  seq 1 1 : (={glob As, glob S, glob O}); 1: by sim.
+  inline {1} 1. inline {2} 2. 
+  swap {2} [2..3] -1.
+  seq 2 2 : (#pre /\ ={glob IdealHSF.RF, rho}). 
+  + by inline *; sim.
+  seq 1 2 : (#pre /\ sig{1} = PRF_.PRF.k{2});1: by inline *; auto => />.
+  inline {1} 1; inline {2} 1.
+  sim 8 8.
+  seq 7 7 : (#pre /\ ={a,rho0} /\ sig0{1} = PRF_.PRF.k{2}); 1: by  sim. 
+  conseq => />.
+  inline {1} 1; inline {2} 1. 
+  inline *. 
+  unroll for {1} 8.
+  unroll for {2} 8.
+  do 3!( wp; conseq => />; sim).
+  wp;auto => />;sim.
+  unroll for {1} 6.
+  unroll for {2} 6.
+  do 3!( wp; conseq => />; sim).
+  by wp;auto => />;sim.
+
+have -> : Pr[CPAGameROM(CPA, KyberSIdeal(DummyHS(IdealHSF.RF), S, KNS, DummyPRF1(IdealPRF1.RF), KPRF), As, O).main() @ &m : res] = 
+          Pr[PRF_DEFS.IND(IdealPRF1.RF, D_PRF1(S, O, As)).main() @ &m : res].
++ byequiv => //.
+  proc. 
+  inline {1} 2; inline {2} 2. inline {2} 2. inline {2} 3.
+  wp; call(_: ={glob O}); 1: by sim.
+  wp; call(_: ={glob O, glob S}); 1: by sim.
+  rnd.
+  wp; call(_: ={glob O}); 1: by sim.
+  conseq (_: _ ==> ={pk, glob O,glob S}); 1: smt().
+  swap {2} 2 -1.
+  seq 1 1 : (={glob As, glob S, glob O}); 1: by sim.
+  inline {1} 1. inline {2} 2. 
+  swap {2} [2..3] -1.
+  seq 2 2 : (#pre /\ ={glob IdealHSF.RF, rho}). 
+  + by inline *; sim.
+  seq 1 2 : (#pre /\ ={glob IdealPRF1.RF,sig});1: by inline *; auto => />.
+  by inline *;sim.
+done.
+qed.
+
+lemma PRFHop2 &m :
+  Pr [ KyberPKE.CPAGameROM(KyberPKE.CPA,KyberSIdeal(DummyHS(IdealHSF.RF),S,KNS,DummyPRF1(IdealPRF1.RF),KPRF),As,O).main() @ &m : res] -
+  Pr [ KyberPKE.CPAGameROM(KyberPKE.CPA,KyberSIdeal(DummyHS(IdealHSF.RF),S,KNS,DummyPRF1(IdealPRF1.RF),DummyPRF2(IdealPRF2.RF)),As,O).main() @ &m : res] = 
+  Pr [ PRF_DEFS.IND(PRF_.PRF,D_PRF2(S,O,As)).main() @ &m : res ] - 
+  Pr [ PRF_DEFS.IND(IdealPRF2.RF,D_PRF2(S,O,As)).main() @ &m : res ].
+proof.
+have -> : Pr[CPAGameROM(CPA, KyberSIdeal(DummyHS(IdealHSF.RF), S, KNS, DummyPRF1(IdealPRF1.RF), KPRF), As, O).main() @ &m : res] = 
+          Pr[PRF_DEFS.IND(PRF_.PRF, D_PRF2(S, O, As)).main() @ &m : res].
++ byequiv => //.
+  proc. 
+  inline {1} 2; inline {2} 2. inline {2} 2. inline {2} 3.
+  wp; call(_: ={glob O}); 1: by sim.
+  swap {2} 1 4.
+  seq 4 4 : (={glob S, glob As, glob O,pk,sk,m0,m1} /\ b0{1} = b2{2}).
+  rnd.
+  wp; call(_: ={glob O}); 1: by sim.
+  wp; call(_: ={glob O, glob S}); 1: by sim.
+  by inline *; auto => />; sim. 
+  conseq (_: _ ==> ={c, glob O,glob S}); 1: smt().
+  inline {1} 1. inline {2} 2. 
+  swap {2} [2..3] -1; sp 2 2.
+  seq 1 2 : (#pre /\ r{1} = PRF_.PRF.k{2});1: by inline *; auto => />.
+  inline {1} 1; inline {2} 1.
+  sim 13 13.
+  seq 12 12 : (={that, m2, aT, glob S, glob O}  /\ r0{1} = PRF_.PRF.k{2}); 1: by  sim. 
+  conseq => />.
+  inline {1} 1; inline {2} 1. 
+  inline *. 
+  wp;auto => />;sim.
+  unroll for {1} 8.
+  unroll for {2} 8.
+  do 3!( wp; conseq => />; sim).
+  wp;auto => />;sim.
+  unroll for {1} 6.
+  unroll for {2} 6.
+  do 3!( wp; conseq => />; sim).
+  by wp;auto => />;sim.
+
+have -> : Pr[CPAGameROM(CPA, KyberSIdeal(DummyHS(IdealHSF.RF), S, KNS, DummyPRF1(IdealPRF1.RF), DummyPRF2(RF)), As, O).main
+   () @ &m : res] = 
+          Pr[PRF_DEFS.IND(RF, D_PRF2(S, O, As)).main() @ &m : res].
++ byequiv => //.
+  proc. 
+  inline {1} 2; inline {2} 2. inline {2} 2. inline {2} 3.
+  wp; call(_: ={glob O}); 1: by sim.
+  swap {2} 1 4.
+  seq 4 4 : (={glob S, glob As, glob O,pk,sk,m0,m1} /\ b0{1} = b2{2}).
+  rnd.
+  wp; call(_: ={glob O}); 1: by sim.
+  wp; call(_: ={glob O, glob S}); 1: by sim.
+  by inline *; auto => />; sim. 
+  conseq (_: _ ==> ={c, glob O,glob S}); 1: smt().
+  inline {1} 1. inline {2} 2. 
+  swap {2} [2..3] -1; sp 2 2.
+  seq 1 2 : (#pre /\ ={glob IdealPRF2.RF,r});1: by inline *; auto => />.
+  by inline *;sim => /> /#.
+done.
+qed.
+
 
 end section.
 
 (*******************************************************************)
+(* At this point we get some nice equivalences                     *)
+(*******************************************************************)
+
+module KyberSI(S : Sampler, O : RO.POracle) = KyberSIdeal(DummyHS(IdealHSF.RF),S,KNS,DummyPRF1(IdealPRF1.RF),DummyPRF2(IdealPRF2.RF), O).
+
+module (NTTSampler(S : Sampler) : Sampler) (O : RO.POracle) = {
+    proc sampleA(sd : W8.t Array32.t) : matrix = { 
+        var a;
+        a <@ S(O).sampleA(sd);
+        return invnttm a;
+    }
+
+    proc sampleAT(sd : W8.t Array32.t) : matrix = { 
+        var a;
+        a <@ S(O).sampleAT(sd);
+        return invnttm a;
+    }
+
+}.
+
+section.
+
+declare module O <: RO.Oracle {-IdealHSF.RF,-RF,-IdealPRF1.RF}.
+declare module S <: Sampler {-IdealHSF.RF,-RF, -O, -IdealPRF1.RF}.
+
+lemma comm_nttv_add v1 v2:  nttv (v1 + v2)%Vector = nttv v1 + nttv v2 by admit.
+lemma comm_nttv_mmul a v: nttv (a *^ v) = ntt_mmul (nttm a) (nttv v) by admit.
+lemma comm_ntt_dotp (v1 v2 : vector): 
+     (MLWE_.(`<*>`) (invnttv v1) v2) = invntt (ntt_dotp v1 (nttv v2)) by admit.
+
+equiv keygen_eq : 
+  MLWE_PKE(NTTSampler(S,O), O).kg ~ KyberSI(S,O).kg :
+   ={glob S, glob O} ==> ={res,glob S, glob O}.
+proof.
+proc.
+inline {2} 4.
+wp;ecall{2}(sem_encode12_vec (toipolyvec s0{2})).
+wp;ecall{2}(sem_encode12_vec (toipolyvec t{2})).
+swap {1} 4 -2.
+swap {2} 2 -1. swap {2} 4 -2. swap {2} 10 -7.
+seq 2 3 : (#pre /\ nttm _A{1} = a{2} /\ sd{1} = rho0{2}).
++ inline {1} 2; wp; call(_: ={glob O}); 1: by sim.
+  by auto => />; smt(nttmK).
+swap {2} [2..3] 4.
+seq 0 5 : #pre; 1: by inline *;auto.
+wp; conseq (_: _ ==> ={e} /\ s{1} = s0{2} /\ sd{1} = rho0{2} /\ nttm _A{1} = a{2}); 
+  last first.
++ conseq (_: true ==> ={e} /\ s{1} = s0{2}); 1: smt(). 
+  admit. (* randomness product *)
+auto => /> &1 &2 e s; rewrite /pk_encode /sk_encode /=.
+by rewrite comm_nttv_add comm_nttv_mmul.
+qed.
+
+equiv enc_eq : 
+  MLWE_PKE(NTTSampler(S,O), O).enc ~ KyberSI(S,O).enc :
+   ={arg,glob S, glob O} ==> ={res,glob S, glob O}.
+proof.
+  proc.
+  inline {2} 2.
+  wp;ecall{2}(sem_encode4 (compress_poly 4 v{2})).
+  wp;ecall{2}(sem_encode10_vec (compress_polyvec 10 u{2})).
+  wp;ecall{2}(sem_decode1 (m0{2})).
+  swap {1} [2..4] -1.
+  swap {2} [7..8] -6.
+  swap {2} 14 -7.
+  swap {2} [6..7] -2.
+  seq 3 5 : (#pre /\ ={e1,e2} /\ r{1} = rv{2}).
+  admit. (* product of randomness *)
+  conseq />; 1: smt().
+  inline {1} 2.
+  swap {2} 3 -2. swap {2} 6 -3. swap {2} 9 -5.
+  seq 4 4 : (#pre /\ tv{2} = pk{1}.`1 /\ t{1} = (pk_decode pk{2}).`1 /\ nttm _A{1} = aT{2}).
+  +  wp; call(_: ={glob O}); 1: by sim.
+     by auto => />; smt(nttmK).
+  wp;ecall{2}(sem_decode12_vec (tv{2})).
+  auto => /> &1 &2; rewrite /pk_decode /c_encode /m_encode /=.  
+  split; 1: by rewrite -comm_nttv_mmul invnttvK.
+  congr. congr. congr. congr.
+  by rewrite comm_ntt_dotp.
+qed.
+ 
+equiv dec_eq : 
+  MLWE_PKE(NTTSampler(S,O), O).dec ~ KyberSI(S,O).dec :
+   ={arg,glob S, glob O} ==> ={res,glob S, glob O}.
+proof.
+  proc.
+  ecall{2} (sem_encode1 (compress_poly 1 mp{2})).
+  wp;ecall{2} (sem_decode12_vec (sk{2})).
+  wp;ecall{2} (sem_decode4 (c2{2})).
+  wp;ecall{2} (sem_decode10_vec (c1{2})).
+  auto => /> &2.
+  rewrite /m_decode /sk_decode /c_decode /=.
+  congr. congr. congr. 
+  by rewrite comm_ntt_dotp.
+qed.
+
+end section.
 
 (***************************************)
 
 section.
 
-declare module O <: RO.Oracle {-KPRF, -B1ROM, -B2ROM}.
-declare module S <: Sampler {-KPRF, -O, -B1ROM, -B2ROM}.
-declare module As <: KyberPKE.AdversaryRO {-O, -S, -KPRF, -B1ROM, -B2ROM}.
+declare module O <: RO.Oracle {-IdealHSF.RF,-IdealPRF1.RF,-RF,-KPRF, -B1ROM, -B2ROM}.
+declare module S <: Sampler {-IdealHSF.RF,-IdealPRF1.RF, -RF, -KPRF, -O, -B1ROM, -B2ROM}.
+declare module As <: KyberPKE.AdversaryRO {-IdealPRF1.RF,-IdealHSF.RF,-RF,-O, -S, -KPRF, -B1ROM, -B2ROM}.
 
 lemma security_any_sampler &m :  
   islossless O.init =>
@@ -618,50 +939,39 @@ lemma security_any_sampler &m :
   (forall (O0 <: RO.Oracle), islossless O0.o => islossless S(O0).sampleAT) =>
   (forall (O0 <: RO.Oracle), islossless O0.o => islossless As(O0).guess) =>
   (forall (O0 <: RO.Oracle), islossless O0.o => islossless As(O0).choose) =>
-  Pr[ KyberPKE.CPAGameROM(KyberPKE.CPA,KyberS(KHS,S,KNS,KPRF),As,O).main() @ &m : res] - 1%r/2%r = 
-  Pr[MLWE_SMP(B1ROM(As, S), S, O).main(false, false) @ &m : res] -
- Pr[MLWE_SMP(B1ROM(As, S), S, O).main(false, true) @ &m : res] +
- Pr[MLWE_SMP(B2ROM(As, S), S, O).main(true, false) @ &m : res] -
- Pr[MLWE_SMP(B2ROM(As, S), S, O).main(true, true) @ &m : res].
+  Pr[ KyberPKE.CPAGameROM(KyberPKE.CPA,KyberSI(S),As,O).main() @ &m : res] - 1%r/2%r = 
+  Pr[MLWE_SMP(B1ROM(As, NTTSampler(S)), NTTSampler(S), O).main(false, false) @ &m : res] -
+ Pr[MLWE_SMP(B1ROM(As, NTTSampler(S)), NTTSampler(S), O).main(false, true) @ &m : res] +
+ Pr[MLWE_SMP(B2ROM(As, NTTSampler(S)), NTTSampler(S), O).main(true, false) @ &m : res] -
+ Pr[MLWE_SMP(B2ROM(As, NTTSampler(S)), NTTSampler(S), O).main(true, true) @ &m : res].
 move => H H0 H1 H2 H3 H4.
 have  <- : 
-    Pr[ PKE_.CPAGameROM(PKE_.CPA,MLWE_PKE(S(O)),As,O).main() @ &m : res] =
-    Pr[ KyberPKE.CPAGameROM(KyberPKE.CPA,KyberS(KHS,S,KNS,KPRF),As,O).main() @ &m : res]; last by
-        apply (main_theorem_s O S As &m  H H0 H1 H2 H3 H4).
+    Pr[ PKE_.CPAGameROM(PKE_.CPA,MLWE_PKE(NTTSampler(S,O)),As,O).main() @ &m : res] =
+    Pr[ KyberPKE.CPAGameROM(KyberPKE.CPA,KyberSI(S),As,O).main() @ &m : res]; last first.
++ apply (main_theorem_s O (NTTSampler(S)) As &m  H H0 _ _ H3 H4).
+  + by move => O0 HH; islossless; apply (H1 O0 HH).
+  by move => O0 HH; islossless; apply (H2 O0 HH). 
 byequiv => //.
 proc.
 inline {1} 2.
 inline {2} 2.
 wp;call(_: ={glob O}); 1: by sim.
-call(_: ={glob S, glob O}).
-(* ENCRYPTION IS EQUIVALENT: Write aux lemma.  *)
-+ inline {2} 2.
-  wp;ecall{2}(sem_encode4 (compress_poly 4 v{2})).
-  wp;ecall{2}(sem_encode10_vec (compress_polyvec 10 u{2})).
-  wp;ecall{2}(sem_decode1 (m0{2})).
-  admit.
-
-rnd;call(_: ={glob O}); 1: by sim.
-conseq />; 1: by smt().
-
-(* KEYGEN IS EQUIVALENT: Write aux lemma.  *)
-call(_: ={glob S, glob O}).
-inline {2} 3. inline {2} 2. 
-wp;ecall{2}(sem_encode12_vec (toipolyvec s0{2})).
-wp;ecall{2}(sem_encode12_vec (toipolyvec t{2})).
-admit.
-
-by inline *; conseq => />; sim.
-
+call (enc_eq O S).
+rnd.
+call(_: ={glob O}); 1: by sim.
+call (keygen_eq O S).
+by conseq />; sim.
 qed.
 
 end section.
 
 section.
 
-declare module O <: RO.Oracle {-KPRF, -B1ROM, -B2ROM}.
-declare module XOF <: XOF_t {-KPRF, -O, -B1ROM, -B2ROM}.
-declare module As <: KyberPKE.AdversaryRO {-O, -XOF, -KPRF, -B1ROM, -B2ROM}.
+
+
+declare module O <: RO.Oracle {-IdealPRF2.RF,-PRF_.PRF,-HSF.PRF,-IdealHSF.RF,-IdealPRF1.RF,-RF,-KPRF, -B1ROM, -B2ROM}.
+declare module XOF <: XOF_t {-IdealPRF2.RF,-PRF_.PRF,-HSF.PRF,-IdealHSF.RF,-IdealPRF1.RF,-RF,-KPRF, -O, -B1ROM, -B2ROM}.
+declare module As <: KyberPKE.AdversaryRO {-IdealPRF2.RF,-PRF_.PRF,-HSF.PRF,-IdealHSF.RF,-IdealPRF1.RF,-RF,-O, -XOF, -KPRF, -B1ROM, -B2ROM}.
 
 (* This theorem yields security for any sampler and we can use
    it to obtain security for the implementation in the standard 
@@ -684,25 +994,40 @@ lemma security_spec &m :
   (forall (O0 <: RO.Oracle), islossless O0.o => islossless As(O0).choose) =>
 
   Pr[ KyberPKE.CPAGameROM(KyberPKE.CPA,Kyber(KHS,XOF,KPRF),As,O).main() @ &m : res] - 1%r/2%r = 
-  Pr[MLWE_SMP(B1ROM(As, KSampler(XOF)),  KSampler(XOF), O).main(false, false) @ &m : res] -
- Pr[MLWE_SMP(B1ROM(As,  KSampler(XOF)),  KSampler(XOF), O).main(false, true) @ &m : res] +
- Pr[MLWE_SMP(B2ROM(As,  KSampler(XOF)),  KSampler(XOF), O).main(true, false) @ &m : res] -
- Pr[MLWE_SMP(B2ROM(As,  KSampler(XOF)),  KSampler(XOF), O).main(true, true) @ &m : res].
+  (Pr [ HS_DEFS.IND(HSF.PRF,D_ES(KSampler(XOF),O,As)).main() @ &m : res ] - 
+  Pr [ HS_DEFS.IND(IdealHSF.RF,D_ES(KSampler(XOF),O,As)).main() @ &m : res ]) +
+  (Pr [ PRF_DEFS.IND(PRF_.PRF,D_PRF1(KSampler(XOF),O,As)).main() @ &m : res ] - 
+  Pr [ PRF_DEFS.IND(IdealPRF1.RF,D_PRF1(KSampler(XOF),O,As)).main() @ &m : res ]) +
+  (Pr [ PRF_DEFS.IND(PRF_.PRF,D_PRF2(KSampler(XOF),O,As)).main() @ &m : res ] - 
+  Pr [ PRF_DEFS.IND(IdealPRF2.RF,D_PRF2(KSampler(XOF),O,As)).main() @ &m : res ]) +
+  (Pr[MLWE_SMP(B1ROM(As, NTTSampler(KSampler(XOF))),  NTTSampler(KSampler(XOF)), O).main(false, false) @ &m : res] -
+ Pr[MLWE_SMP(B1ROM(As,  NTTSampler(KSampler(XOF))),  NTTSampler(KSampler(XOF)), O).main(false, true) @ &m : res] +
+ Pr[MLWE_SMP(B2ROM(As,  NTTSampler(KSampler(XOF))),  NTTSampler(KSampler(XOF)), O).main(true, false) @ &m : res] -
+ Pr[MLWE_SMP(B2ROM(As,  NTTSampler(KSampler(XOF))),  NTTSampler(KSampler(XOF)), O).main(true, true) @ &m : res]).
 move => Oill Ooll XOF_init_ll XOF_next_ll Parse_ll Asgll Ascll.
-have <- : Pr[ KyberPKE.CPAGameROM(KyberPKE.CPA,KyberS(KHS,KSampler(XOF),KNS,KPRF),As,O).main() @ &m : res]= 
-          Pr[ KyberPKE.CPAGameROM(KyberPKE.CPA,Kyber(KHS,XOF,KPRF),As,O).main() @ &m : res];
-  last first.
-+ apply (security_any_sampler O (KSampler(XOF)) As &m Oill Ooll  _ _ Asgll Ascll).
+have <- : Pr[ KyberPKE.CPAGameROM(KyberPKE.CPA,KyberS(KHS,KSampler(XOF),KNS,KPRF,KPRF),As,O).main() @ &m : res]= 
+          Pr[ KyberPKE.CPAGameROM(KyberPKE.CPA,Kyber(KHS,XOF,KPRF),As,O).main() @ &m : res].
++ byequiv => //.
+  proc; inline {1} 2; inline {2} 2.
+  wp; call(_: ={glob O, glob XOF}); 1: by sim.
+  call (enc_sampler_enc O XOF).
+  rnd.
+  wp; call(_: ={glob O, glob XOF}); 1: by sim.
+  call (kg_sampler_kg O XOF).
+  by call(_: true); auto => />. 
+
+have <- := (security_any_sampler O (KSampler(XOF)) As &m Oill Ooll  _ _ Asgll Ascll).
   + by move => O O_ll; apply (KSamplerA_ll XOF O O_ll XOF_init_ll XOF_next_ll Parse_ll).
   by move => O O_ll; apply (KSamplerAT_ll XOF O O_ll XOF_init_ll XOF_next_ll Parse_ll).
-byequiv => //.
-proc; inline {1} 2; inline {2} 2.
-wp; call(_: ={glob O, glob XOF}); 1: by sim.
-call (enc_sampler_enc O XOF).
-rnd.
-wp; call(_: ={glob O, glob XOF}); 1: by sim.
-call (kg_sampler_kg O XOF).
-by call(_: true); auto => />. 
+
+have <- := (ESHop O (KSampler(XOF)) As).
+have <- := (PRFHop1 O (KSampler(XOF)) As).
+have <- := (PRFHop2 O (KSampler(XOF)) As).
+have <- := (KyberS_KyberIdeal O (KSampler(XOF)) As).
+have <-: Pr[CPAGameROM(CPA, KyberSI(KSampler(XOF)), As, O).main() @ &m : res] = 
+         Pr[CPAGameROM(CPA, KyberSIdeal(DummyHS(IdealHSF.RF), KSampler(XOF), KNS, DummyPRF1(IdealPRF1.RF), DummyPRF2(RF)), As, O).main
+   () @ &m : res] by byequiv => //=; proc; sim.
+by ring.
 qed.
 
 end section.
@@ -722,9 +1047,9 @@ section.
 module O = MLWE_.MLWE_ROM.RO_H.Lazy.LRO.
 module OS =RO.Lazy.LRO.
 
-declare module As <: KyberPKE.AdversaryRO {-O, -OS, -KPRF, -B1ROM, -B2ROM, -B,-Bt, -BS, -D, -LazyEager.ERO}.
-declare module S <: Sampler {-As, -B1ROM, -B2ROM, -OS, -O, -B,-Bt, -BS, -D, -LazyEager.ERO}.
-declare module Sim <: Simulator_t {-S,-As,-B1ROM, -B2ROM, -OS, -O, -B,-Bt, -BS, -D, -LazyEager.ERO}.
+declare module As <: KyberPKE.AdversaryRO {-IdealPRF1.RF,-IdealHSF.RF,-RF,-O, -OS, -KPRF, -B1ROM, -B2ROM, -B,-Bt, -BS, -D, -LazyEager.ERO}.
+declare module S <: Sampler {-IdealPRF1.RF,-IdealHSF.RF,-RF,-As, -B1ROM, -B2ROM, -OS, -O, -B,-Bt, -BS, -D, -LazyEager.ERO}.
+declare module Sim <: Simulator_t {-IdealPRF1.RF,-IdealHSF.RF,-S,-As,-B1ROM, -B2ROM, -OS, -O, -B,-Bt, -BS, -D, -LazyEager.ERO}.
 
 lemma security_any_sampler_indiff &m :  
   (forall (x : RO.in_t), is_lossless (RO.dout x)) => 
@@ -734,44 +1059,32 @@ lemma security_any_sampler_indiff &m :
   (forall (O <: RO.Oracle), islossless O.o => islossless As(O).choose) =>
 
   (forall tr b (D0 <: Distinguisher_t {-S,-Sim,-O,-OS}),
-     Pr[ WIndfReal(D0,S,OS).main(tr,b) @ &m : res] = 
+     Pr[ WIndfReal(D0,NTTSampler(S),OS).main(tr,b) @ &m : res] = 
      Pr[ WIndfIdeal(D0,Sim,O).main(tr,b) @ &m : res]) =>
 
-  Pr[ KyberPKE.CPAGameROM(KyberPKE.CPA,KyberS(KHS,S,KNS,KPRF),As,OS).main() @ &m : res] - 1%r/2%r = 
-    Pr[MLWE(B(BS(B1ROM(As,S),Sim),RO_H.Lazy.LRO)).main(false) @ &m : res] -
-       Pr[MLWE(B(BS(B1ROM(As,S),Sim),RO_H.Lazy.LRO)).main(true) @ &m : res] + 
-    Pr[MLWE(Bt(BS(B2ROM(As,S),Sim),RO_H.Lazy.LRO)).main(false) @ &m : res]-
-       Pr[MLWE(Bt(BS(B2ROM(As,S),Sim),RO_H.Lazy.LRO)).main(true) @ &m : res].
+  Pr[ KyberPKE.CPAGameROM(KyberPKE.CPA,KyberSI(S),As,OS).main() @ &m : res] - 1%r/2%r = 
+    Pr[MLWE(B(BS(B1ROM(As,NTTSampler(S)),Sim),RO_H.Lazy.LRO)).main(false) @ &m : res] -
+       Pr[MLWE(B(BS(B1ROM(As,NTTSampler(S)),Sim),RO_H.Lazy.LRO)).main(true) @ &m : res] + 
+    Pr[MLWE(Bt(BS(B2ROM(As,NTTSampler(S)),Sim),RO_H.Lazy.LRO)).main(false) @ &m : res]-
+       Pr[MLWE(Bt(BS(B2ROM(As,NTTSampler(S)),Sim),RO_H.Lazy.LRO)).main(true) @ &m : res].
 move => H H0 H1 H2 H3 H4.
 have  <- : 
-    Pr[ PKE_.CPAGameROM(PKE_.CPA,MLWE_PKE(S(OS)),As,OS).main() @ &m : res] =
-    Pr[ KyberPKE.CPAGameROM(KyberPKE.CPA,KyberS(KHS,S,KNS,KPRF),As,OS).main() @ &m : res]; 
-     last by apply (main_theorem_ref As S Sim &m  H H0 H1 H2 H3 H4).
-byequiv => //.
-proc.
-inline {1} 2.
-inline {2} 2.
-wp;call(_: ={glob OS}); 1: by sim.
-call(_: ={glob S, glob OS}).
-(* ENCRYPTION IS EQUIVALENT: Write aux lemma.  *)
-+ inline {2} 2.
-  wp;ecall{2}(sem_encode4 (compress_poly 4 v{2})).
-  wp;ecall{2}(sem_encode10_vec (compress_polyvec 10 u{2})).
-  wp;ecall{2}(sem_decode1 (m0{2})).
-  admit.
+    Pr[ PKE_.CPAGameROM(PKE_.CPA,MLWE_PKE(NTTSampler(S,OS)),As,OS).main() @ &m : res] =
+    Pr[ KyberPKE.CPAGameROM(KyberPKE.CPA,KyberSI(S),As,OS).main() @ &m : res].
++ byequiv => //.
+  proc.
+  inline {1} 2.
+  inline {2} 2.
+  wp;call(_: ={glob OS}); 1: by sim.
+  call (enc_eq OS S).
+  rnd.
+  call(_: ={glob OS}); 1: by sim.
+  call (keygen_eq OS S).
+  by conseq />; sim.
 
-rnd;call(_: ={glob OS}); 1: by sim.
-conseq />; 1: by smt().
-
-(* KEYGEN IS EQUIVALENT: Write aux lemma.  *)
-call(_: ={glob S, glob OS}).
-inline {2} 3. inline {2} 2.
-wp;ecall{2}(sem_encode12_vec (toipolyvec s0{2})).
-wp;ecall{2}(sem_encode12_vec (toipolyvec t{2})).
-admit.
-
-by inline *; conseq => />; sim.
-
+apply (main_theorem_ref As (NTTSampler(S)) Sim &m  H _ _ H2 H3 H4).
++ by move => O0 HH; islossless; apply (H0 O0 HH).
+by move => O0 HH; islossless; apply (H1 O0 HH).
 qed.
 
 end section.
@@ -794,9 +1107,9 @@ end section.
 
 section.
 
-declare module As <: KyberPKE.AdversaryRO {-O, -OS, -KPRF, -B1ROM, -B2ROM, -B,-Bt, -BS, -D, -LazyEager.ERO}.
-declare module XOF <: XOF_t {-As, -B1ROM, -B2ROM, -OS, -O, -B,-Bt, -BS, -D, -LazyEager.ERO}.
-declare module Sim <: Simulator_t {-XOF,-As,-B1ROM, -B2ROM, -OS, -O, -B,-Bt, -BS, -D, -LazyEager.ERO}.
+declare module As <: KyberPKE.AdversaryRO {-IdealPRF2.RF,-PRF_.PRF,-HSF.PRF,-IdealHSF.RF,-IdealPRF1.RF,-O, -OS, -KPRF, -B1ROM, -B2ROM, -B,-Bt, -BS, -D, -LazyEager.ERO}.
+declare module XOF <: XOF_t {-IdealPRF2.RF,-PRF_.PRF,-HSF.PRF,-IdealHSF.RF,-IdealPRF1.RF,-As, -B1ROM, -B2ROM, -OS, -O, -B,-Bt, -BS, -D, -LazyEager.ERO}.
+declare module Sim <: Simulator_t {-IdealPRF2.RF,-PRF_.PRF,-HSF.PRF,-IdealHSF.RF,-IdealPRF1.RF,-XOF,-As,-B1ROM, -B2ROM, -OS, -O, -B,-Bt, -BS, -D, -LazyEager.ERO}.
 
 lemma security_spec_indiff &m :  
   (forall (x : RO.in_t), is_lossless (RO.dout x)) => 
@@ -813,44 +1126,62 @@ lemma security_spec_indiff &m :
   (forall (O0 <: RO.Oracle), islossless O0.o => islossless As(O0).choose) =>
 
   (forall tr b (D0 <: Distinguisher_t {-KSampler(XOF),-Sim,-O,-OS}),
-     Pr[ WIndfReal(D0,KSampler(XOF),OS).main(tr,b) @ &m : res] = 
+     Pr[ WIndfReal(D0,NTTSampler(KSampler(XOF)),OS).main(tr,b) @ &m : res] = 
      Pr[ WIndfIdeal(D0,Sim,O).main(tr,b) @ &m : res]) =>
 
 
   Pr[ KyberPKE.CPAGameROM(KyberPKE.CPA,Kyber(KHS,XOF,KPRF),As,OS).main() @ &m : res] - 1%r/2%r = 
-    Pr[MLWE(B(BS(B1ROM(As,KSampler(XOF)),Sim),RO_H.Lazy.LRO)).main(false) @ &m : res] -
-       Pr[MLWE(B(BS(B1ROM(As,KSampler(XOF)),Sim),RO_H.Lazy.LRO)).main(true) @ &m : res] + 
-    Pr[MLWE(Bt(BS(B2ROM(As,KSampler(XOF)),Sim),RO_H.Lazy.LRO)).main(false) @ &m : res]-
-       Pr[MLWE(Bt(BS(B2ROM(As,KSampler(XOF)),Sim),RO_H.Lazy.LRO)).main(true) @ &m : res].
+  (Pr [ HS_DEFS.IND(HSF.PRF,D_ES(KSampler(XOF),OS,As)).main() @ &m : res ] - 
+  Pr [ HS_DEFS.IND(IdealHSF.RF,D_ES(KSampler(XOF),OS,As)).main() @ &m : res ]) +
+  (Pr [ PRF_DEFS.IND(PRF_.PRF,D_PRF1(KSampler(XOF),OS,As)).main() @ &m : res ] - 
+  Pr [ PRF_DEFS.IND(IdealPRF1.RF,D_PRF1(KSampler(XOF),OS,As)).main() @ &m : res ]) +
+  (Pr [ PRF_DEFS.IND(PRF_.PRF,D_PRF2(KSampler(XOF),OS,As)).main() @ &m : res ] - 
+  Pr [ PRF_DEFS.IND(IdealPRF2.RF,D_PRF2(KSampler(XOF),OS,As)).main() @ &m : res ]) +
+  (Pr[MLWE(B(BS(B1ROM(As,NTTSampler(KSampler(XOF))),Sim),RO_H.Lazy.LRO)).main(false) @ &m : res] -
+       Pr[MLWE(B(BS(B1ROM(As,NTTSampler(KSampler(XOF))),Sim),RO_H.Lazy.LRO)).main(true) @ &m : res] + 
+    Pr[MLWE(Bt(BS(B2ROM(As,NTTSampler(KSampler(XOF))),Sim),RO_H.Lazy.LRO)).main(false) @ &m : res]-
+       Pr[MLWE(Bt(BS(B2ROM(As,NTTSampler(KSampler(XOF))),Sim),RO_H.Lazy.LRO)).main(true) @ &m : res]).
 
 move => Oill XOF_init_ll XOF_next_ll Parse_ll Asgll Ascll ind.
-have <- : Pr[ KyberPKE.CPAGameROM(KyberPKE.CPA,KyberS(KHS,KSampler(XOF),KNS,KPRF),As,OS).main() @ &m : res]= 
-          Pr[ KyberPKE.CPAGameROM(KyberPKE.CPA,Kyber(KHS,XOF,KPRF),As,OS).main() @ &m : res];
-  last first.
-+ apply (security_any_sampler_indiff  As (KSampler(XOF)) Sim  &m Oill _ _ Asgll Ascll ind).
+have <- : Pr[ KyberPKE.CPAGameROM(KyberPKE.CPA,KyberS(KHS,KSampler(XOF),KNS,KPRF,KPRF),As,OS).main() @ &m : res]= 
+          Pr[ KyberPKE.CPAGameROM(KyberPKE.CPA,Kyber(KHS,XOF,KPRF),As,OS).main() @ &m : res].
++ byequiv => //.
+  proc; inline {1} 2; inline {2} 2.
+  wp; call(_: ={glob OS, glob XOF}); 1: by sim.
+  call (enc_sampler_enc OS XOF).
+  rnd.
+  wp; call(_: ={glob OS, glob XOF}); 1: by sim.
+  call (kg_sampler_kg OS XOF).
+  by inline *; auto.
+
++ have <- := (security_any_sampler_indiff  As (KSampler(XOF)) Sim  &m Oill _ _ Asgll Ascll ind).
   + by move => O O_ll; apply (KSamplerA_ll XOF O O_ll XOF_init_ll XOF_next_ll Parse_ll).
   by move => O O_ll; apply (KSamplerAT_ll XOF O O_ll XOF_init_ll XOF_next_ll Parse_ll).
-byequiv => //.
-proc; inline {1} 2; inline {2} 2.
-wp; call(_: ={glob OS, glob XOF}); 1: by sim.
-call (enc_sampler_enc OS XOF).
-rnd.
-wp; call(_: ={glob OS, glob XOF}); 1: by sim.
-call (kg_sampler_kg OS XOF).
-by inline *; auto.
+
+have <- := (ESHop OS (KSampler(XOF)) As).
+have <- := (PRFHop1 OS (KSampler(XOF)) As).
+have <- := (PRFHop2 OS (KSampler(XOF)) As).
+have <- := (KyberS_KyberIdeal OS (KSampler(XOF)) As).
+have <-: Pr[CPAGameROM(CPA, KyberSI(KSampler(XOF)), As, OS).main() @ &m : res] = 
+         Pr[CPAGameROM(CPA, KyberSIdeal(DummyHS(IdealHSF.RF), KSampler(XOF), KNS, DummyPRF1(IdealPRF1.RF), DummyPRF2(RF)), As, OS).main
+   () @ &m : res] by byequiv => //=; proc; sim.
+by ring.
 qed.
+
 
 end section.
 
 (* The correctness bounds can only be computed when matrices are
    uniform, so we jump directly to results where one can assume
-   that the sampler is indifferentiable from the nice RO *)
+   that the sampler is indifferentiable from the nice RO.
+   Note here we are working with the scheme with ideal HS and
+   PRFs. *)
 
 section.
 
-declare module A <: CAdversaryRO {-O,-OS}.
-declare module S <: Sampler {-A,-O,-OS}.
-declare module Sim <: Simulator_t {-S, -A,-O,-OS}.
+declare module A <: CAdversaryRO {-IdealPRF1.RF,-IdealHSF.RF,-O,-OS}.
+declare module S <: Sampler {-IdealPRF1.RF,-IdealHSF.RF,-A,-O,-OS}.
+declare module Sim <: Simulator_t {-IdealPRF1.RF,-IdealHSF.RF,-S, -A,-O,-OS}.
 
 
 lemma correctness_any_sampler &m epsilon_hack fail_prob :
@@ -858,7 +1189,7 @@ lemma correctness_any_sampler &m epsilon_hack fail_prob :
   (forall (O <: RO.POracle), islossless O.o => islossless A(O).find) =>
 
   (forall trb (D0 <: Distinguisher_t {-S,-Sim,-SMP_vs_ROM_IND.O,-SMP_vs_ROM_IND.OS}),
-     Pr[ WIndfReal(D0,S,OS).main(trb) @ &m : res] = 
+     Pr[ WIndfReal(D0,NTTSampler(S),OS).main(trb) @ &m : res] = 
      Pr[ WIndfIdeal(D0,Sim,O).main(trb) @ &m : res]) =>
 
 (* This jump is assumed to introduce no slack in the
@@ -869,55 +1200,252 @@ lemma correctness_any_sampler &m epsilon_hack fail_prob :
 (* The following failure probability can be bounded as
 in the Python script for Kyber *)   
   Pr[ CorrectnessBound.main() @ &m : res] <= fail_prob =>
-  Pr[ KyberPKE.CorrectnessAdvROM(KyberS(KHS,S,KNS,KPRF),A,OS).main() @ &m : res]  >=
+  Pr[ KyberPKE.CorrectnessAdvROM(KyberSI(S),A,OS).main() @ &m : res]  >=
   1%r - fail_prob - epsilon_hack.
 move => Sim_ll A_ll ind eh nb.
 have <- : 
-Pr[PKE_.CGameROM(PKE_.CorrectnessAdv, MLWE_PKE(S(RO.Lazy.LRO)), A, RO.Lazy.LRO).main() @ &m : res] = 
-Pr[CorrectnessAdvROM(KyberS(KHS, S, KNS,KPRF), A, OS).main() @ &m : res]; 
-   last by apply (correctness_bound A S Sim &m epsilon_hack fail_prob Sim_ll A_ll ind eh nb).
+Pr[PKE_.CGameROM(PKE_.CorrectnessAdv, MLWE_PKE(NTTSampler(S,RO.Lazy.LRO)), A, RO.Lazy.LRO).main() @ &m : res] = 
+Pr[CorrectnessAdvROM(KyberSI(S), A, OS).main() @ &m : res]; 
+   last by apply (correctness_bound A (NTTSampler(S)) Sim &m epsilon_hack fail_prob Sim_ll A_ll ind eh nb).
 byequiv => //.
 proc.
 inline {1} 2; inline {2} 2.
-wp;call(_: ={glob S, glob OS}).
-(* Decryption is EQUIVALENT: Write Aux Lemma *)
-+ wp;ecall{2}(sem_encode1 (compress_poly 1 mp{2})).
-  wp;ecall{2}(sem_decode12_vec (sk{2})).
-  wp;ecall{2}(sem_decode4 (c2{2})).
-  wp;ecall{2}(sem_decode10_vec (c1{2})).
-  auto => /> *. 
-  rewrite /m_decode /c_decode; congr; congr => /=; congr.
-  admit. (* Hugo : bring in ntt properties *)
-
-call(_: ={glob S, glob OS}).
-(* ENCRYPTION IS EQUIVALENT: Write aux lemma.  *)
-+ inline {2} 2.
-  wp;ecall{2}(sem_encode4 (compress_poly 4 v{2})).
-  wp;ecall{2}(sem_encode10_vec (compress_polyvec 10 u{2})).
-  admit.
-
-call(_: ={glob OS}); 1: by sim.
-
-(* KEYGEN IS EQUIVALENT: Write aux lemma.  *)
-call(_: ={glob S, glob OS}).
-inline {2} 3. inline {2} 2.
-wp;ecall{2}(sem_encode12_vec (toipolyvec s0{2})).
-wp;ecall{2}(sem_encode12_vec (toipolyvec t{2})).
-admit. 
-
-by inline *; conseq => />;  auto => />.
+wp;call (dec_eq (RO.Lazy.LRO) S).
+wp;call (enc_eq (RO.Lazy.LRO) S).
+call(_: ={glob S, glob OS}); 1: by sim.
+wp;call (keygen_eq (RO.Lazy.LRO) S).
+by conseq => />; sim.
 qed. 
 
 end section.
 
-(* For the full spec we ge the following result, which does 
-   not require losslessness, but does require indifferentiability. *)
+(* For the full spec we get the following result, which does 
+   not require losslessness, but does require indifferentiability. 
+   However we must first game hop to the ideal scheme. *)
+
+module (DC_ES(S : Sampler, O : RO.Oracle, Ac : KyberPKE.CAdversaryRO) : HS_DEFS.Distinguisher) (F : HS_DEFS.PRF_Oracles)  = {
+
+    proc distinguish() : bool = {
+       var b;
+       b <@ KyberPKE.CorrectnessAdvROM(KyberS(DummyHS_D(F),S,KNS,KPRF,KPRF),Ac,O).main();
+       return b;
+    } 
+}.
+
+module (DC_PRF1(S : Sampler, O : RO.Oracle, Ac : KyberPKE.CAdversaryRO) : PRF_DEFS.Distinguisher) (F : PRF_DEFS.PRF_Oracles)  = {
+
+    proc distinguish() : bool = {
+       var b;
+       b <@ KyberPKE.CorrectnessAdvROM(KyberSIdeal(DummyHS(IdealHSF.RF),S,KNS,DummyPRF1(F),KPRF),Ac,O).main();
+       return b;
+    } 
+}.
+
+module (DC_PRF2(S : Sampler, O : RO.Oracle, Ac : KyberPKE.CAdversaryRO) : PRF_DEFS.Distinguisher) (F : PRF_DEFS.PRF_Oracles)  = {
+
+    proc distinguish() : bool = {
+       var b;
+       b <@ KyberPKE.CorrectnessAdvROM(KyberSIdeal(DummyHS(IdealHSF.RF),S,KNS,DummyPRF1(IdealPRF1.RF),DummyPRF2D(F)),Ac,O).main();
+       return b;
+    } 
+}.
 
 section.
 
-declare module A <: CAdversaryRO {-O,-OS}.
-declare module XOF <: XOF_t {-A,-O,-OS}.
-declare module Sim <: Simulator_t {-XOF, -A,-O,-OS}.
+declare module O <: RO.Oracle {-IdealPRF2.RF, -IdealPRF1.RF, -PRF_.PRF, -IdealHSF.RF, -KPRF, -B1ROM, -B2ROM, -HSF.PRF}.
+declare module S <: Sampler {-IdealPRF2.RF, -IdealPRF1.RF, -PRF_.PRF, -IdealHSF.RF, -KPRF, -O, -B1ROM, -B2ROM}.
+declare module Ac <: KyberPKE.CAdversaryRO {-IdealPRF2.RF, -IdealPRF1.RF, -PRF_.PRF, -IdealHSF.RF, -HSF.PRF, -O, -S, -KPRF, -B1ROM, -B2ROM}.
+
+lemma ESHopC &m :
+  Pr [ KyberPKE.CorrectnessAdvROM(KyberS(KHS,S,KNS,KPRF,KPRF),Ac,O).main() @ &m : res] -
+  Pr [ KyberPKE.CorrectnessAdvROM(KyberS(DummyHS(IdealHSF.RF),S,KNS,KPRF,KPRF),Ac,O).main() @ &m : res] = 
+  Pr [ HS_DEFS.IND(HSF.PRF,DC_ES(S,O,Ac)).main() @ &m : res ] - 
+  Pr [ HS_DEFS.IND(IdealHSF.RF,DC_ES(S,O,Ac)).main() @ &m : res ].
+proof.
+have -> : Pr[CorrectnessAdvROM(KyberS(KHS, S, KNS, KPRF,KPRF), Ac, O).main() @ &m : res]  = 
+          Pr[HS_DEFS.IND(HSF.PRF, DC_ES(S, O, Ac)).main() @ &m : res] .
++ byequiv => //.
+  proc. 
+  inline {1} 2; inline {2} 2. inline {2} 2. inline {2} 3.
+  wp; call(_: ={glob O, glob S}); 1: by sim.
+  wp; call(_: ={glob O, glob S}); 1: by sim.
+  wp; call(_: ={glob O}); 1: by sim.
+  conseq (_: _ ==> ={pk,sk, glob O,glob S}); 1: smt().
+  swap {2} 2 -1.
+  seq 1 1 : (={glob Ac, glob S, glob O}); 1: by sim.
+  inline {1} 1. inline {1} 1. inline {2} 2. inline {2} 1.
+  seq 3 3 : (#pre /\ ={rho,sig}); 1: by inline *; sim.
+  by sim.
+
++ have -> : 
+    Pr[CorrectnessAdvROM(KyberS(DummyHS(IdealHSF.RF), S, KNS, KPRF, KPRF), Ac, O).main() @ &m : res] = 
+    Pr[HS_DEFS.IND(IdealHSF.RF, DC_ES(S, O, Ac)).main() @ &m : res].
++ byequiv => //.
+  proc. 
+  inline {1} 2; inline {2} 2. inline {2} 2. inline {2} 3.
+  wp; call(_: ={glob O, glob S}); 1: by sim.
+  wp; call(_: ={glob O, glob S}); 1: by sim.
+  wp; call(_: ={glob O}); 1: by sim.
+  conseq (_: _ ==> ={pk,sk, glob O,glob S}); 1: smt().
+  swap {2} 2 -1.
+  seq 1 1 : (={glob Ac, glob S, glob O}); 1: by sim.
+  inline {1} 1. inline {1} 1. inline {2} 2. inline {2} 1.
+  seq 3 3 : (#pre /\ ={rho,sig}); 1: by inline *; sim.
+  by sim.
+done.
+qed.
+
+lemma KyberS_KyberIdeal_C &m :
+  Pr [ CorrectnessAdvROM(KyberS(DummyHS(IdealHSF.RF),S,KNS,KPRF,KPRF),Ac,O).main() @ &m : res] =
+  Pr [ CorrectnessAdvROM(KyberSIdeal(DummyHS(IdealHSF.RF),S,KNS,KPRF,KPRF),Ac,O).main() @ &m : res].
+proof.
+byequiv => //.
+proc. 
+  inline {1} 2; inline {2} 2. 
+  wp; call(_: ={glob O, glob S}); 1: by sim.
+  wp; call(_: ={glob O, glob S}); 1: by sim.
+  wp; call(_: ={glob O}); 1: by sim.
+  conseq (_: _ ==> ={pk,sk, glob O,glob S}); 1: smt().
+  seq 1 1 : (={glob Ac, glob S, glob O}); 1: by sim.
+  inline {1} 1. inline {2} 1. 
+  wp; call(_: ={glob O, glob S}); 1: by sim.
+  conseq => />.
+  inline *.
+  rcondt{1} 6; 1: by move => *; auto => />;smt(@SmtMap).
+  seq {1} 5 2 : (true); 1: by auto.
+  wp.
+  conseq (_: _ ==> rho{2} = Array32.init (fun i => r{1}.[i]) /\ 
+                   k{2} = Array32.init (fun i => r{1}.[i+32]));
+  1: by move => /> [#] &1 r; 
+       rewrite !SmtMap.get_set_sameE !oget_some.
+  admit. (* Product of distributions *)
+qed.
+
+lemma PRFHop1C &m :
+  Pr [ CorrectnessAdvROM(KyberSIdeal(DummyHS(IdealHSF.RF),S,KNS,KPRF,KPRF),Ac,O).main() @ &m : res] -
+  Pr [ CorrectnessAdvROM(KyberSIdeal(DummyHS(IdealHSF.RF),S,KNS,DummyPRF1(IdealPRF1.RF),KPRF),Ac,O).main() @ &m : res] = 
+  Pr [ PRF_DEFS.IND(PRF_.PRF,DC_PRF1(S,O,Ac)).main() @ &m : res ] - 
+  Pr [ PRF_DEFS.IND(IdealPRF1.RF,DC_PRF1(S,O,Ac)).main() @ &m : res ].
+proof.
+have -> : Pr[CorrectnessAdvROM(KyberSIdeal(DummyHS(IdealHSF.RF), S, KNS, KPRF, KPRF), Ac, O).main() @ &m : res] = 
+          Pr[PRF_DEFS.IND(PRF_.PRF, DC_PRF1(S, O, Ac)).main() @ &m : res].
++ byequiv => //.
+  proc. 
+  inline {1} 2; inline {2} 2. inline {2} 2. inline {2} 3.
+  wp; call(_: ={glob O, glob S}); 1: by sim.
+  wp; call(_: ={glob O, glob S}); 1: by sim.
+  wp; call(_: ={glob O}); 1: by sim.
+  conseq (_: _ ==> ={pk, sk,glob O,glob S}); 1: smt().
+  swap {2} 2 -1.
+  seq 1 1 : (={glob Ac, glob S, glob O}); 1: by sim.
+  inline {1} 1. inline {2} 2. 
+  swap {2} [2..3] -1.
+  seq 2 2 : (#pre /\ ={glob IdealHSF.RF, rho}). 
+  + by inline *; sim.
+  seq 1 2 : (#pre /\ sig{1} = PRF_.PRF.k{2});1: by inline *; auto => />.
+  inline {1} 1; inline {2} 1.
+  sim 8 8.
+  seq 7 7 : (#pre /\ ={a,rho0} /\ sig0{1} = PRF_.PRF.k{2}); 1: by  sim. 
+  conseq => />.
+  inline {1} 1; inline {2} 1. 
+  inline *. 
+  unroll for {1} 8.
+  unroll for {2} 8.
+  do 3!( wp; conseq => />; sim).
+  wp;auto => />;sim.
+  unroll for {1} 6.
+  unroll for {2} 6.
+  do 3!( wp; conseq => />; sim).
+  by wp;auto => />;sim.
+
+have -> : Pr[CorrectnessAdvROM(KyberSIdeal(DummyHS(IdealHSF.RF), S, KNS, DummyPRF1(IdealPRF1.RF), KPRF), Ac, O).main() @ &m : res] = 
+          Pr[PRF_DEFS.IND(IdealPRF1.RF, DC_PRF1(S, O, Ac)).main() @ &m : res].
++ byequiv => //.
+  proc. 
+  inline {1} 2; inline {2} 2. inline {2} 2. inline {2} 3.
+  wp; call(_: ={glob O, glob S}); 1: by sim.
+  wp; call(_: ={glob O, glob S}); 1: by sim.
+  wp; call(_: ={glob O}); 1: by sim.
+  conseq (_: _ ==> ={pk, sk, glob O,glob S}); 1: smt().
+  swap {2} 2 -1.
+  seq 1 1 : (={glob Ac, glob S, glob O}); 1: by sim.
+  inline {1} 1. inline {2} 2. 
+  swap {2} [2..3] -1.
+  seq 2 2 : (#pre /\ ={glob IdealHSF.RF, rho}). 
+  + by inline *; sim.
+  seq 1 2 : (#pre /\ ={glob IdealPRF1.RF,sig});1: by inline *; auto => />.
+  by inline *;sim.
+done.
+qed.
+
+lemma PRFHop2C &m :
+  Pr [ CorrectnessAdvROM(KyberSIdeal(DummyHS(IdealHSF.RF),S,KNS,DummyPRF1(IdealPRF1.RF),KPRF),Ac,O).main() @ &m : res] -
+  Pr [ CorrectnessAdvROM(KyberSIdeal(DummyHS(IdealHSF.RF),S,KNS,DummyPRF1(IdealPRF1.RF),DummyPRF2(IdealPRF2.RF)),Ac,O).main() @ &m : res] = 
+  Pr [ PRF_DEFS.IND(PRF_.PRF,DC_PRF2(S,O,Ac)).main() @ &m : res ] - 
+  Pr [ PRF_DEFS.IND(IdealPRF2.RF,DC_PRF2(S,O,Ac)).main() @ &m : res ].
+proof.
+have -> : Pr[CorrectnessAdvROM(KyberSIdeal(DummyHS(IdealHSF.RF), S, KNS, DummyPRF1(IdealPRF1.RF), KPRF), Ac, O).main() @ &m : res] = 
+          Pr[PRF_DEFS.IND(PRF_.PRF, DC_PRF2(S, O, Ac)).main() @ &m : res].
++ byequiv => //.
+  proc. 
+  inline {1} 2; inline {2} 2. inline {2} 2. inline {2} 3.
+  wp; call(_: ={glob O, glob S}); 1: by sim.
+  swap {2} 1 3.
+  seq 3 3 : (={glob S, glob Ac, glob O,pk,sk,m}).
+  + wp; call(_: ={glob O}); 1: by sim.
+    wp; call(_: ={glob O, glob S}); 1: by sim.
+    by inline *; auto => />; sim. 
+  conseq (_: _ ==> ={c, glob O,glob S}); 1: smt().
+  inline {1} 1. inline {2} 2. 
+  swap {2} [2..3] -1; sp 2 2.
+  seq 1 2 : (#pre /\ r{1} = PRF_.PRF.k{2});1: by inline *; auto => />.
+  inline {1} 1; inline {2} 1.
+  sim 13 13.
+  seq 12 12 : (={that, m1, aT, glob S, glob O}  /\ r0{1} = PRF_.PRF.k{2}); 1: by  sim. 
+  conseq => />.
+  inline {1} 1; inline {2} 1. 
+  inline *. 
+  wp;auto => />;sim.
+  unroll for {1} 8.
+  unroll for {2} 8.
+  do 3!( wp; conseq => />; sim).
+  wp;auto => />;sim.
+  unroll for {1} 6.
+  unroll for {2} 6.
+  do 3!( wp; conseq => />; sim).
+  by wp;auto => />;sim.
+
+have -> : Pr[CorrectnessAdvROM(KyberSIdeal(DummyHS(IdealHSF.RF), S, KNS, DummyPRF1(IdealPRF1.RF), DummyPRF2(RF)), Ac, O).main
+   () @ &m : res] = 
+          Pr[PRF_DEFS.IND(RF, DC_PRF2(S, O, Ac)).main() @ &m : res].
++ byequiv => //.
+  proc. 
+  inline {1} 2; inline {2} 2. inline {2} 2. inline {2} 3.
+  wp; call(_: ={glob O, glob S}); 1: by sim.
+  swap {2} 1 3.
+  seq 3 3 : (={glob S, glob Ac, glob O,pk,sk,m}).
+  + wp; call(_: ={glob O}); 1: by sim.
+    wp; call(_: ={glob O, glob S}); 1: by sim.
+    by inline *; auto => />; sim. 
+  conseq (_: _ ==> ={c, glob O,glob S}); 1: smt().
+  inline {1} 1. inline {2} 2. 
+  swap {2} [2..3] -1; sp 2 2.
+  seq 1 2 : (#pre /\ ={glob IdealPRF2.RF,r});1: by inline *; auto => />.
+  by inline *;sim => /> /#.
+done.
+qed.
+
+
+end section.
+
+
+section.
+
+
+
+declare module A <: CAdversaryRO {-HSF.PRF, -PRF_.PRF, -B1ROM, -B2ROM, -KPRF, -RF,-IdealHSF.RF, -IdealPRF1.RF, -O,-OS}.
+declare module XOF <: XOF_t {-HSF.PRF, -PRF_.PRF, -B1ROM, -B2ROM, -KPRF, -RF,-IdealHSF.RF, -IdealPRF1.RF, -A,-O,-OS}.
+declare module Sim <: Simulator_t {-HSF.PRF, -PRF_.PRF, -B1ROM, -B2ROM, -KPRF, -RF,-IdealHSF.RF, -IdealPRF1.RF, -XOF, -A,-O,-OS}.
 
 
 lemma correctness_spec &m epsilon_hack fail_prob :
@@ -925,7 +1453,7 @@ lemma correctness_spec &m epsilon_hack fail_prob :
   (forall (O <: RO.POracle), islossless O.o => islossless A(O).find) =>
 
   (forall trb (D0 <: Distinguisher_t {-KSampler(XOF),-Sim,-SMP_vs_ROM_IND.O,-SMP_vs_ROM_IND.OS}),
-     Pr[ WIndfReal(D0,KSampler(XOF),OS).main(trb) @ &m : res] = 
+     Pr[ WIndfReal(D0,NTTSampler(KSampler(XOF)),OS).main(trb) @ &m : res] = 
      Pr[ WIndfIdeal(D0,Sim,O).main(trb) @ &m : res]) =>
 
 (* This jump is assumed to introduce no slack in the
@@ -937,38 +1465,39 @@ lemma correctness_spec &m epsilon_hack fail_prob :
 in the Python script for Kyber *)   
   Pr[ CorrectnessBound.main() @ &m : res] <= fail_prob =>
   Pr[ KyberPKE.CorrectnessAdvROM(Kyber(KHS,XOF,KPRF),A,OS).main() @ &m : res]  >=
-  1%r - fail_prob - epsilon_hack.
+  1%r - fail_prob - epsilon_hack -
+  (`|Pr [ HS_DEFS.IND(HSF.PRF,DC_ES(KSampler(XOF),OS,A)).main() @ &m : res ] - 
+  Pr [ HS_DEFS.IND(IdealHSF.RF,DC_ES(KSampler(XOF),OS,A)).main() @ &m : res ]|) -
+  (`|Pr [ PRF_DEFS.IND(PRF_.PRF,DC_PRF1(KSampler(XOF),OS,A)).main() @ &m : res ] - 
+  Pr [ PRF_DEFS.IND(IdealPRF1.RF,DC_PRF1(KSampler(XOF),OS,A)).main() @ &m : res ]|) -
+  (`|Pr [ PRF_DEFS.IND(PRF_.PRF,DC_PRF2(KSampler(XOF),OS,A)).main() @ &m : res ] - 
+  Pr [ PRF_DEFS.IND(IdealPRF2.RF,DC_PRF2(KSampler(XOF),OS,A)).main() @ &m : res ]|).
 move => Sim_ll A_ll ind eh fp.
-have <-: Pr[CorrectnessAdvROM(KyberS(KHS, KSampler(XOF), KNS,KPRF), A, OS).main() @ &m : res] = 
-         Pr[CorrectnessAdvROM(Kyber(KHS, XOF, KPRF), A, OS).main() @ &m : res];
-  last by apply (correctness_any_sampler A (KSampler(XOF)) Sim &m).
-byequiv => //.
-proc. 
-inline {1} 2; inline {2} 2.
-wp; call(_: ={glob OS, glob XOF}); 1: by sim.
-call (enc_sampler_enc OS XOF).
-wp; call(_: ={glob OS}); 1: by sim.
-call (kg_sampler_kg OS XOF).
-by inline *; auto.
+have <-: Pr[CorrectnessAdvROM(KyberS(KHS, KSampler(XOF), KNS,KPRF,KPRF), A, OS).main() @ &m : res] = 
+         Pr[CorrectnessAdvROM(Kyber(KHS, XOF, KPRF), A, OS).main() @ &m : res].
++ byequiv => //.
+  proc. 
+  inline {1} 2; inline {2} 2.
+  wp; call(_: ={glob OS, glob XOF}); 1: by sim.
+  call (enc_sampler_enc OS XOF).
+  wp; call(_: ={glob OS}); 1: by sim.
+  call (kg_sampler_kg OS XOF).
+  by inline *; auto.
+
+move : (correctness_any_sampler A (KSampler(XOF)) Sim &m epsilon_hack fail_prob Sim_ll A_ll ind eh fp).
+
+have <- := (ESHopC OS (KSampler(XOF)) A).
+have <- := (PRFHop1C OS (KSampler(XOF)) A).
+have <- := (PRFHop2C OS (KSampler(XOF)) A).
+have <- := (KyberS_KyberIdeal_C OS (KSampler(XOF)) A).
+have <-: Pr[CorrectnessAdvROM(KyberSI(KSampler(XOF)), A, OS).main() @ &m : res] = 
+         Pr[CorrectnessAdvROM(KyberSIdeal(DummyHS(IdealHSF.RF), KSampler(XOF), KNS, DummyPRF1(IdealPRF1.RF), DummyPRF2(RF)), A, OS).main
+   () @ &m : res] by byequiv => //=; proc; sim.
+
+
+by smt().
 qed.
 
 end section.
 
 end SpecProperties.
-
-
-theory ImplementationProperties.
-
-(* To Do: Get the equivalence results from 
-   correctness folder INDCPA and show by
-   transitivity that implementation is correct
-   and secure because of the theorems above.
-   The challenge will come from matching 
-   the used G, PRF and XOF: a blunt approach
-   is to assume functional equivalence for
-   these components, which is fine for everything
-   except the XOF, which actually uses a RO
-   in the security and correctness analyses.
- *)
-
-end ImplementationProperties.
